Source/DafnyRuntime/DafnyRuntimeJs/Concurrent.dfy
@@ -1,70 +1,67 @@
 
-module  {:extern} {:compile false} Std.JavaScriptConcurrent replaces Concurrent {
+/**
+Dafny-native implementation, possible because JavaScript is single threadded 
+*/
+module Std.JavaScriptConcurrent replaces Concurrent {
 
-  class {:extern} MutableMap<K(==), V(==)> ... {
+  class Lock ... {
 
-    constructor {:extern} {:axiom} (ghost inv: (K, V) -> bool)
-
-    ghost predicate Valid()
-    {
-      true
+    constructor() {
+      isLocked := false;
     }
 
-    method {:extern} {:axiom} Keys() returns (keys: set<K>)
+    method Lock()
+    {
+      // Written this way so that we don't get a warning about
+      // "requires !isLocked" being an unnecessary precondition.
+      isLocked := !isLocked;
+    }
 
-    method {:extern} {:axiom} HasKey(k: K) returns (used: bool)
-
-    method {:extern} {:axiom} Values() returns (values: set<V>)
-
-    method {:extern} {:axiom} Items() returns (items: set<(K,V)>)
-
-    method {:extern} {:axiom} Put(k: K, v: V)
-
-    method {:extern} {:axiom} Get(k: K) returns (r: Option<V>)
-
-    method {:extern} {:axiom} Remove(k: K)
-
-    method {:extern} {:axiom} Size() returns (c: nat)
+    method Unlock()
+    {
+      // Written this way so that we don't get a warning about
+      // "requires isLocked" being an unnecessary precondition.
+      isLocked := !isLocked;
+    }
 
   }
 
-  class {:extern} AtomicBox<T> ... {
+  class AtomicBox<T> ... {
 
-    constructor {:extern} {:axiom} (ghost inv: T -> bool, t: T)
+    var boxed: T
 
-    ghost predicate Valid() { true }
+    ghost predicate Valid()
+      reads this 
+    {
+      this.inv(boxed)
+    }
 
-    method {:extern} {:axiom} Get() returns (t: T)
+    constructor (ghost inv: T -> bool, t: T)
+    {
+      boxed := t;
+      this.inv := inv;
+    }
 
-    method {:extern} {:axiom} Put(t: T)
+    method Get() returns (t: T)
+    {
+      t := boxed;
+    }
+
+    method Put(t: T)
+    {
+      boxed := t;
+    }
 
   }
 
-  class {:extern} Lock ... {
+  class MutableMap<K(==), V(==)> ... {
 
-    constructor {:extern} {:axiom} ()
-
-    method {:extern} {:axiom} Lock()
-
-    method {:extern} {:axiom} Unlock()
-
-  }
-}
-
-// Dafny-native implementation, used to generate the extern implementation
-module Std.ConcurrentDafny {
-
-  import opened Wrappers
-
-  class MutableMap<K(==), V(==)> {
-
-    ghost const inv: (K, V) -> bool
     ghost var knownKeys: set<K>
     ghost var knownValues: set<V>
 
     var internal: map<K, V>
 
-    constructor (inv: (K, V) -> bool)
+    constructor (ghost inv: (K, V) -> bool)
       ensures Valid()
       ensures this.inv == inv
     {
@@ -81,55 +78,39 @@ module Std.ConcurrentDafny {
     }
 
     ghost predicate Valid()
-      reads this
     {
       forall k :: k in internal.Keys ==> inv(k, internal[k]) && Contained()
     }
 
     method Keys() returns (keys: set<K>)
-      requires Valid()
-      ensures forall k :: k in keys ==> exists v :: v in knownValues && inv(k,v)
     {
       reveal Contained();
       keys := internal.Keys;
     }
 
     method HasKey(k: K) returns (used: bool)
-      requires Valid()
-      ensures used ==> exists v :: v in knownValues && inv(k,v)
     {
       reveal Contained();
       used := k in internal.Keys;
     }
 
     method Values() returns (values: set<V>)
-      requires Valid()
-      ensures forall v :: v in values ==> exists k :: k in knownKeys && inv(k,v)
     {
       reveal Contained();
       values := internal.Values;
     }
 
     method Items() returns (items: set<(K,V)>)
-      requires Valid()
-      ensures forall t :: t in items ==> inv(t.0, t.1)
     {
       items := internal.Items;
     }
 
     method Get(k: K) returns (r: Option<V>)
-      requires Valid()
-      ensures r.Some? ==> inv(k, r.value)
     {
       r := if k in internal.Keys then Some(internal[k]) else None;
     }
 
     method Put(k: K, v: V)
-      requires Valid()
-      requires inv(k, v)
-      modifies this
-      ensures Valid()
-
     {
       internal := internal[k := v];
       knownKeys := knownKeys + {k};
@@ -138,10 +119,6 @@ module Std.ConcurrentDafny {
     }
 
     method Remove(k: K)
-      requires Valid()
-      requires exists v :: inv(k,v)
-      modifies this
-      ensures Valid()
     {
       // only here to mollify the auditor
       assert exists v :: inv(k,v);
@@ -151,7 +128,6 @@ module Std.ConcurrentDafny {
     }
 
     method Size() returns (c: nat)
-      requires Valid()
     {
       // only here to mollify the auditor
       reveal Contained();
@@ -161,73 +137,4 @@ module Std.ConcurrentDafny {
     }
 
   }
-
-  class AtomicBox<T> {
-
-    ghost const inv: T -> bool
-
-    var boxed: T
-
-    constructor (inv: T -> bool, t: T)
-      requires inv(t)
-      ensures Valid()
-      ensures this.inv == inv
-    {
-      boxed := t;
-      this.inv := inv;
-    }
-
-    ghost predicate Valid()
-      reads this
-    {
-      inv(boxed)
-    }
-
-    method Get() returns (t: T)
-      requires Valid()
-      ensures inv(t)
-    {
-      t := boxed;
-    }
-
-    method Put(t: T)
-      requires inv(t)
-      modifies this
-      ensures Valid()
-    {
-      boxed := t;
-    }
-
-  }
-
-  class Lock {
-
-    ghost var isLocked: bool
-
-    constructor() {
-      isLocked := false;
-    }
-
-    method Lock()
-      requires !isLocked
-      modifies this
-      ensures isLocked
-    {
-      // Written this way so that we don't get a warning about
-      // "requires !isLocked" being an unnecessary precondition.
-      isLocked := !isLocked;
-    }
-
-    method Unlock()
-      requires isLocked
-      modifies this
-      ensures !isLocked
-    {
-      // Written this way so that we don't get a warning about
-      // "requires isLocked" being an unnecessary precondition.
-      isLocked := !isLocked;
-    }
-
-  }
-
 }
